theories/Lambda/ExprUnify_common.v
@@ -1,0 +1,330 @@
+Require Import ExtLib.Core.RelDec.
+Require Import ExtLib.Data.HList.
+Require Import ExtLib.Data.Option.
+Require Import ExtLib.Data.Fun.
+Require Import ExtLib.Data.Eq.
+Require Import ExtLib.Tactics.
+Require Import MirrorCore.EnvI.
+Require Import MirrorCore.ExprI.
+Require Import MirrorCore.SymI.
+Require Import MirrorCore.SubstI.
+Require Import MirrorCore.TypesI.
+Require Import MirrorCore.Lambda.ExprCore.
+Require Import MirrorCore.Lambda.ExprD.
+Require Import MirrorCore.Lambda.ExprLift.
+Require Import MirrorCore.Lambda.ExprTac.
+Require Import MirrorCore.Util.Forwardy.
+
+Require Import FunctionalExtensionality.
+
+Set Implicit Arguments.
+Set Strict Implicit.
+
+Section typed.
+  Variable subst : Type.
+  Variable typ : Type.
+  Variable func : Type.
+  Variable RType_typ : RType typ.
+  Variable RTypeOk_typ : RTypeOk.
+  Variable Typ2_arr : Typ2 _ Fun.
+  Variable Typ2Ok_arr : Typ2Ok Typ2_arr.
+  Variable RSym_func : RSym func.
+  Variable RSymOk_func : RSymOk RSym_func.
+  Variable Subst_subst : Subst subst (expr typ func).
+  Variable SubstUpdate_subst : SubstUpdate subst (expr typ func).
+  Variable SubstOk_subst : SubstOk (Expr_expr) Subst_subst.
+  Variable SubstUpdateOk_subst
+  : @SubstUpdateOk _ _ _ _ Expr_expr _ SubstUpdate_subst _.
+  Local Instance Expr_expr : Expr _ (expr typ func) := Expr_expr.
+
+  Lemma handle_set
+  : forall (e0 : expr typ func) (u : uvar) (s s' : subst)
+    (Hnot_found : lookup u s = None),
+      set u e0 s = Some s' ->
+      WellFormed_subst s ->
+      WellFormed_subst s' /\
+      forall (tu : tenv typ) (tv : list typ)
+             (t : typ) (tv' : list typ),
+        (forall
+            (v1 : _)
+            (v2 : hlist (typD nil) tu ->
+                    hlist (typD nil) (tv' ++ tv) -> typD nil t)
+            (sD : hlist (typD nil) tu -> hlist (typD nil) tv -> Prop),
+            exprD' nil tu tv t e0 = Some v1 ->
+            exprD' nil tu (tv' ++ tv) t (UVar u) = Some v2 ->
+            substD tu tv s = Some sD ->
+            exists
+              sD' : hlist (typD nil) tu -> hlist (typD nil) tv -> Prop,
+              substD tu tv s' = Some sD' /\
+              (forall (us : hlist (typD nil) tu)
+                      (vs : hlist (typD nil) tv),
+                 sD' us vs ->
+                 sD us vs /\
+                 (forall vs' : hlist (typD nil) tv',
+                    v1 us vs = v2 us (hlist_app vs' vs)))).
+  Proof.
+    intros.
+    eapply set_sound in H; eauto.
+    forward_reason; split; eauto.
+    intros.
+    autorewrite with exprD_rw in *; eauto. simpl in *.
+    forwardy.
+    destruct y.
+    specialize (H1 _ _ _ _ _ _ H4 H3 H2).
+    forward_reason.
+    eexists; split; eauto.
+    intros.
+    eapply H7 in H8; forward_reason; split; auto.
+    intros. rewrite <- H9.
+    inv_all; subst. reflexivity.
+  Qed.
+
+  Lemma handle_set_lower
+  : forall (e0 : expr typ func) (u : uvar) (s s' : subst)
+           (Hnot_found : lookup u s = None),
+      set u e0 s = Some s' ->
+      WellFormed_subst s ->
+      WellFormed_subst s' /\
+      forall (tu : tenv typ) (tv : list typ)
+             (t : typ) (tv' : list typ) (e : expr typ func),
+        lower 0 (length tv') e = Some e0 ->
+        (forall
+            (v1
+               v2 : hlist (typD nil) tu ->
+                    hlist (typD nil) (tv' ++ tv) -> typD nil t)
+            (sD : hlist (typD nil) tu -> hlist (typD nil) tv -> Prop),
+            exprD' nil tu (tv' ++ tv) t e = Some v1 ->
+            exprD' nil tu (tv' ++ tv) t (UVar u) = Some v2 ->
+            substD tu tv s = Some sD ->
+            exists
+              sD' : hlist (typD nil) tu -> hlist (typD nil) tv -> Prop,
+              substD tu tv s' = Some sD' /\
+              (forall (us : hlist (typD nil) tu)
+                      (vs : hlist (typD nil) tv),
+                 sD' us vs ->
+                 sD us vs /\
+                 (forall vs' : hlist (typD nil) tv',
+                    v1 us (hlist_app vs' vs) = v2 us (hlist_app vs' vs)))).
+  Proof.
+    intros.
+    eapply set_sound in H; eauto.
+    forward_reason; split; eauto.
+    intros.
+    autorewrite with exprD_rw in *; simpl in *.
+    forwardy.
+    destruct y. inv_all; subst.
+    eapply  (@exprD'_lower typ func _ _ RSym_func _ _ _ nil tu nil tv' tv) in H2; eauto.
+    forward_reason.
+    specialize (H1 _ _ _ _ _ _ H5 H4 H2).
+    forward_reason.
+    eexists; split; eauto.
+    intros.
+    eapply H8 in H9; clear H8.
+    forward_reason; split; eauto.
+    rewrite H9. intros. eapply (H7 us Hnil vs' vs).
+  Qed.
+
+  Definition unify_sound_ind
+    (unify : forall ts (us vs : tenv typ) (under : nat) (s : subst)
+                    (l r : expr typ func)
+                    (t : typ), option subst) : Prop :=
+    forall tu tv e1 e2 s s' t tv',
+      unify (@nil Type) tu (tv' ++ tv) (length tv') s e1 e2 t = Some s' ->
+      WellFormed_subst (expr := expr typ func) s ->
+      WellFormed_subst (expr := expr typ func) s' /\
+      forall v1 v2 sD,
+        exprD' nil tu (tv' ++ tv) t e1 = Some v1 ->
+        exprD' nil tu (tv' ++ tv) t e2 = Some v2 ->
+        substD tu tv s = Some sD ->
+        exists sD',
+             substD (expr := expr typ func) tu tv s' = Some sD'
+          /\ forall us vs,
+               sD' us vs ->
+               sD us vs /\
+               forall vs',
+                 v1 us (hlist_app vs' vs) = v2 us (hlist_app vs' vs).
+
+  Definition unify_sound := unify_sound_ind.
+
+  Lemma handle_uvar
+  : forall
+      (unify : list Type -> tenv typ -> tenv typ ->
+               nat -> subst -> expr typ func -> expr typ func -> typ -> option subst),
+      unify_sound_ind unify ->
+      forall (tu : tenv typ) (tv : list typ) e
+             (u : uvar) (s s' : subst) (t : typ) (tv' : list typ),
+        match lookup u s with
+          | Some e2' =>
+            unify nil tu (tv' ++ tv) (length tv') s e
+                  (lift 0 (length tv') e2') t
+          | None =>
+            match lower 0 (length tv') e with
+              | Some e1 => set u e1 s
+              | None => None
+            end
+        end = Some s' ->
+        WellFormed_subst s ->
+        WellFormed_subst s' /\
+        (forall
+            (v1 v2 : hlist (typD nil) tu ->
+                     hlist (typD nil) (tv' ++ tv) -> typD nil t)
+            (sD : hlist (typD nil) tu -> hlist (typD nil) tv -> Prop),
+            exprD' nil tu (tv' ++ tv) t e = Some v1 ->
+            exprD' nil tu (tv' ++ tv) t (UVar u) = Some v2 ->
+            substD tu tv s = Some sD ->
+            exists
+              sD' : hlist (typD nil) tu -> hlist (typD nil) tv -> Prop,
+              substD tu tv s' = Some sD' /\
+              (forall (us : hlist (typD nil) tu) (vs : hlist (typD nil) tv),
+                 sD' us vs ->
+                 sD us vs /\
+                 (forall vs' : hlist (typD nil) tv',
+                    v1 us (hlist_app vs' vs) = v2 us (hlist_app vs' vs)))).
+  Proof.
+    intros.
+    consider (lookup u s); intros.
+    { eapply H in H2.
+      forward_reason.
+      split; eauto; intros.
+      assert (exists v2',
+                exprD' nil tu (tv' ++ tv) t (lift 0 (length tv') e0) = Some v2'
+                /\ forall us vs vs',
+                     sD us vs ->
+                     v2 us (hlist_app vs' vs) = v2' us (hlist_app vs' vs)).
+      { eapply substD_lookup in H0; eauto.
+        forward_reason.
+        simpl in *.
+        autorewrite with exprD_rw in H5; simpl in H5.
+        forward. inv_all; subst.
+        change_rewrite H5 in H9. inv_all; subst.
+        eapply nth_error_get_hlist_nth_Some in H5.
+        simpl in *. forward_reason.
+        generalize (@exprD'_lift typ func _ _ _ _ _ _ nil tu e0 nil tv' tv x2).
+        simpl. change_rewrite H7.
+        intros; forwardy. destruct r.
+        eexists; split; [ eassumption | ].
+        intros.
+        erewrite H8; try eassumption.
+        specialize (H9 us Hnil vs' vs).
+        simpl in H9.
+        rewrite H9.
+        reflexivity. }
+      forward_reason.
+      specialize (H3 _ _ _ H4 H7 H6).
+      forward_reason.
+      eexists; split; eauto.
+      intros. specialize (H9 _ _ H10).
+      forward_reason. split; intros; eauto.
+      rewrite H11. rewrite H8; eauto. }
+    { forward. eapply handle_set_lower in H3; intuition eauto. }
+  Qed.
+
+  Lemma handle_uvar'
+  : forall
+        unify : list Type -> tenv typ -> tenv typ ->
+                nat -> subst -> expr typ func -> expr typ func -> typ -> option subst,
+        unify_sound_ind unify ->
+        forall (tu : tenv typ) (tv : list typ) e
+               (u : uvar) (s s' : subst) (t : typ) (tv' : list typ),
+          match lookup u s with
+            | Some e2' =>
+              unify nil tu (tv' ++ tv) (length tv') s
+                    (lift 0 (length tv') e2') e t
+            | None =>
+              match lower 0 (length tv') e with
+                | Some e1 => set u e1 s
+                | None => None
+              end
+          end = Some s' ->
+          WellFormed_subst s ->
+          WellFormed_subst s' /\
+          (forall
+              (v1 v2 : hlist (typD nil) tu ->
+                       hlist (typD nil) (tv' ++ tv) -> typD nil t)
+              (sD : hlist (typD nil) tu -> hlist (typD nil) tv -> Prop),
+              exprD' nil tu (tv' ++ tv) t (UVar u) = Some v1 ->
+              exprD' nil tu (tv' ++ tv) t e = Some v2 ->
+              substD tu tv s = Some sD ->
+              exists
+                sD' : hlist (typD nil) tu -> hlist (typD nil) tv -> Prop,
+                substD tu tv s' = Some sD' /\
+                (forall (us : hlist (typD nil) tu)
+                        (vs : hlist (typD nil) tv),
+                   sD' us vs ->
+                   sD us vs /\
+                   (forall vs' : hlist (typD nil) tv',
+                      v1 us (hlist_app vs' vs) = v2 us (hlist_app vs' vs)))).
+  Proof.
+    intros.
+    consider (lookup u s); intros.
+    { eapply H in H2.
+      forward_reason.
+      split; eauto; intros.
+      assert (exists v2',
+                exprD' nil tu (tv' ++ tv) t (lift 0 (length tv') e0) = Some v2'
+                /\ forall us vs vs',
+                     sD us vs ->
+                     v1 us (hlist_app vs' vs) = v2' us (hlist_app vs' vs)).
+      { eapply substD_lookup in H0; eauto.
+        forward_reason.
+        simpl in *.
+        autorewrite with exprD_rw in H4; simpl in H4.
+        forwardy. inv_all; subst.
+        change_rewrite H0 in H4.
+        inv_all; subst.
+        generalize (@exprD'_lift typ func _ _ _ _ _ _ nil tu e0 nil tv' tv x).
+        simpl. change_rewrite H7.
+        intros; forwardy.
+        destruct y.
+        eexists; split; [ eassumption | ].
+        intros.
+        specialize (H10 us Hnil vs' vs).
+        specialize (H8 us vs).
+        simpl in *.
+        etransitivity; [ clear H10 | exact H10 ].
+        apply H8. assumption. }
+      forward_reason.
+      specialize (H3 _ _ _ H7 H5 H6).
+      forward_reason.
+      eexists; split; eauto.
+      intros. specialize (H9 _ _ H10).
+      forward_reason. split; intros; eauto.
+      rewrite H8; eauto. }
+    { forwardy. eapply handle_set_lower in H3; intuition eauto.
+      specialize (H5 _ _ _ _ _ H2 _ _ _ H6 H3 H7).
+      forward_reason. eexists; split; eauto.
+      intros. specialize (H8 _ _ H9). forward_reason; split; eauto. }
+  Qed.
+
+  Lemma lookup_lift
+  : forall u s e tu tv tv' t sD v1,
+      lookup u s = Some e ->
+      WellFormed_subst s ->
+      substD tu tv s = Some sD ->
+      exprD' nil tu (tv' ++ tv) t (UVar u) = Some v1 ->
+      exists v1',
+        exprD' nil tu (tv' ++ tv) t (lift 0 (length tv') e) = Some v1' /\
+        forall us vs vs',
+          sD us vs ->
+          v1 us (hlist_app vs' vs) = v1' us (hlist_app vs' vs).
+  Proof.
+    intros.
+    eapply substD_lookup in H; eauto.
+    simpl in *. forward_reason.
+    generalize (@exprD'_lift typ func RType_typ Typ2_arr _ _ _ _
+                             nil tu e nil tv' tv x).
+    simpl. change_rewrite H3.
+    intros; forwardy.
+    autorewrite with exprD_rw in H2. simpl in H2.
+    change_rewrite H in H2.
+    forwardy.
+    inv_all. subst. destruct y0.
+    eexists; split; [ eapply H5 | ].
+    clear - H4 H6.
+    intros.
+    specialize (H6 us Hnil vs' vs).
+    simpl in *.
+    etransitivity; [ eapply H4 | eapply H6 ]; eauto.
+  Qed.
+
+End typed.
